DynamoDbEncryption/dafny/DynamoDbEncryption/src/Beacon.dfy
@@ -39,6 +39,9 @@ module BaseBeacon {
     nameonly beaconName: DDB.AttributeName
   ) {
 
+    //= specification/searchable-encryption/beacons.md#basichash
+    //= type=implication
+    //# * basicHash MUST take an [hmac key](./search-config.md#hmac-key-generation), a [beacon length](#beacon-length) and a sequence of bytes as input.
     function method {:opaque} hash(val : Bytes, key : Bytes, length : BeaconLength)
       : (ret : Result<string, Error>)
       ensures ret.Success? ==>
@@ -79,6 +82,15 @@ module BaseBeacon {
     // calculate the HMAC for some bytes
     function method {:opaque} getHmac(data : Bytes, key : Bytes) : (res : Result<Bytes, Error>)
       ensures res.Success? ==> |res.value| == 8
+
+      ensures res.Success? ==>
+                //= specification/searchable-encryption/beacons.md#basichash
+                //= type=implication
+                //# * basicHash MUST calculate the [HmacSha384](https://www.ietf.org/rfc/rfc2104.txt)
+                //# of the input bytes and the [hmac key](./search-config.md#hmac-key-generation), and keep the first 8 bytes.
+                && var input := Prim.HMacInput(digestAlgorithm := Prim.SHA_384, key := key, message := data);
+                && client.HMac(input).Success?
+                && res.value == client.HMac(input).value[..8]
     {
       var input := Prim.HMacInput (
                      digestAlgorithm := Prim.SHA_384,
@@ -98,7 +110,10 @@ module BaseBeacon {
     length : BeaconLength,
     loc : string
   )
-    : Result<ValidStandardBeacon, Error>
+    : (ret : Result<ValidStandardBeacon, Error>)
+    ensures ret.Success? ==>
+              && TermLoc.MakeTermLoc(loc).Success?
+              && ret.value.loc == TermLoc.MakeTermLoc(loc).value
   {
     var termLoc :- TermLoc.MakeTermLoc(loc);
     var beaconName := BeaconPrefix + name;
@@ -142,7 +157,26 @@ module BaseBeacon {
         hash(str.value, keys[base.name])
     }
 
-    function method {:opaque} getHash(item : DDB.AttributeMap, vf : VirtualFieldMap, key : Bytes) : Result<Option<string>, Error>
+    //= specification/searchable-encryption/beacons.md#value-for-a-standard-beacon
+    //= type=implication
+    //# * This operation MUST take an [hmac key](./search-config.md#hmac-key-generation), a record as input, and produce an optional string.
+    function method {:opaque} getHash(item : DDB.AttributeMap, vf : VirtualFieldMap, key : Bytes) : (ret : Result<Option<string>, Error>)
+      ensures ret.Success? ==>
+                && VirtToBytes(loc, item, vf).Success?
+                   //= specification/searchable-encryption/beacons.md#value-for-a-standard-beacon
+                   //= type=implication
+                   //# * This operation MUST convert the attribute value of the associated field to
+                   //# a sequence of bytes, as per [attribute serialization](../dynamodb-encryption-client/ddb-attribute-serialization.md).
+                && var bytes := VirtToBytes(loc, item, vf).value;
+                //= specification/searchable-encryption/beacons.md#value-for-a-standard-beacon
+                //= type=implication
+                //# * This operation MUST return no value if the associated field does not exist in the record
+                && (bytes.None? ==> ret.value.None?)
+                   //= specification/searchable-encryption/beacons.md#value-for-a-standard-beacon
+                   //= type=implication
+                   //# * This operation MUST return the [basicHash](#basichash) of the input and the configured [beacon length](#beacon-length).
+                && (bytes.Some? ==> ret.value.Some? && hash(bytes.value, key).Success? && ret.value.value == hash(bytes.value, key).value)
+                && (bytes.Some? ==> ret.value.Some? && base.hash(bytes.value, key, length).Success? && ret.value.value == base.hash(bytes.value, key, length).value)
     {
       var bytes :- VirtToBytes(loc, item, vf);
       if bytes.None? then
@@ -172,6 +206,9 @@ module BaseBeacon {
       Success(DDB.AttributeValue.S(h))
     }
 
+    //= specification/searchable-encryption/beacons.md#getpart-for-a-standard-beacon
+    //= type=implication
+    //# * getPart MUST take an [hmac key](./search-config.md#hmac-key-generation), a sequence of bytes as input, and produce a string.
     function method {:opaque} getPart(val : Bytes, key : Bytes)
       : (ret : Result<string, Error>)
       requires 0 < |val|
