specification/searchable-encryption/beacons.md
@@ -307,7 +307,7 @@ This name MUST match the name of one of the [sensitive](#sensitive-part-initiali
 
 * If no constructors are configured, a default constructor MUST be generated.
 * This default constructor MUST be all of the non-sensitive parts,
-followed by all the sensitive part, all parts being required.
+followed by all the sensitive parts, all parts being required.
 
 ### Part
 
@@ -319,8 +319,7 @@ Initialization MUST fail if any `prefix` in any [part](#part) is a prefix of
 the `prefix` of any other [part](#part).
 
 Initialization MUST fail if any [non-sensitive-part](#non-sensitive-part-initialization) contains
-any part of an encrypted field, or any [sensitive-part](#sensitive-part-initialization) fails to contain
-some part of an encrypted field.
+anything but SIGN_ONLY fields.
 
 Initialization MUST fail if any [constructor](#constructor) is configured with a field name
 that is not a defined [part](#part).
@@ -367,7 +366,7 @@ a sequence of bytes, as per [attribute serialization](../dynamodb-encryption-cli
 on the `split character`,
 excluding parts that are not required and with a source field that is not available.
  * This operation MUST fail if any plaintext value used in the construction contains the split character.
- * If no constructor, this operation must return no value.
+ * If no constructor succeeds, this operation MUST return no value.
 
 ### getPart for a standard beacon
 
@@ -397,7 +396,7 @@ The `Part Value` is the [part value calculation](#part-value-calculation) of the
 ### Part Value Calculation
 
 Part Value Calculation MUST take an [hmac key](./search-config.md#hmac-key-generation), a string, a prefix,
-and an optional [beacon length](#beacon-length) as input, and return a string as output.
+and a [Part](#part) as input, and return a string as output.
 
 The input string MUST begin with the provided prefix.
 
